src/3d/GenMakefile.fsti
@@ -2,5 +2,6 @@ module GenMakefile
 
 val write_gnu_makefile
   (skip_o_rules: bool)
+  (clang_format: bool)
   (files: list string)
 : FStar.All.ML unit
